src/Examples/ExMach/RefinementAdequacy.v
@@ -5,7 +5,6 @@ From iris.algebra Require Export functions.
 From iris.base_logic.lib Require Export invariants gen_heap.
 From iris.proofmode Require Export tactics.
 Require Export ExMach.ExMachAPI ExMach.WeakestPre.
-Set Default Proof Using "Type".
 
 Class exmachPreG Σ := ExMachPreG {
   exm_preG_iris :> invPreG Σ;
@@ -232,7 +231,15 @@ Section refinement.
   Notation recover := impl.(recover).
   Notation compile_proc_seq := impl.(compile_proc_seq).
   Context `{exmachPreG Σ}.
-  Context (φinv: forall {_ : @cfgG OpT Λa Σ} {_ : exmachG Σ}, iProp Σ).
+  Context `{cfgPreG OpT Λa Σ}.
+  Context (crash_inner: forall {_ : @cfgG OpT Λa Σ} {_: exmachG Σ}, iProp Σ).
+  Context (exec_inner: forall {_ : @cfgG OpT Λa Σ} {_ : exmachG Σ}, iProp Σ).
+  Context (crash_inv: forall {_ : @cfgG OpT Λa Σ} {_ : exmachG Σ}, iProp Σ).
+  Context (exec_inv: forall {_ : @cfgG OpT Λa Σ} {_ : exmachG Σ}, iProp Σ).
+
+  Context (einv_persist: forall {H1 : @cfgG OpT Λa Σ} {H2 : exmachG Σ}, Persistent (exec_inv H1 H2)).
+  Context (cinv_persist: forall {H1 : @cfgG OpT Λa Σ} {H2 : exmachG Σ}, Persistent (crash_inv H1 H2)).
+
   Context (E: coPset).
   Context (nameIncl: nclose sourceN ⊆ E).
   (* TODO: we should get rid of rec_seq if we're not exploiting vertical comp anymore *)
@@ -241,28 +248,317 @@ Section refinement.
 
   Context (refinement_triples:
              forall {H1 H2 T1 T2} j K `{LanguageCtx OpT T1 T2 Λa K} (e: proc OpT T1),
-               j ⤇ K e ∗ (@φinv H1 H2) ⊢
+               j ⤇ K e ∗ (@exec_inv H1 H2) ⊢
                  WP compile e {{ v, j ⤇ K (Ret v) }}).
 
   Context (recv_triple:
              forall {H1 H2},
-               (@φinv H1 H2) ⊢
+               (@crash_inv H1 H2) ⊢
                     WP recv @ NotStuck; ⊤ {{ v, |={⊤,E}=> ∃ σ2a σ2a', source_state σ2a
-                                               ∗ ⌜Λa.(crash_step) σ2a (Val σ2a' tt)⌝}}).
+                    ∗ ⌜Λa.(crash_step) σ2a (Val σ2a' tt)⌝ ∗
+                    ∀ `{Hcfg': cfgG OpT Λa Σ} (Hinv': invG Σ) ρ,
+                      source_ctx (ρ, σ2a') ∗ source_state σ2a'  ={⊤}=∗
+                      exec_inner Hcfg' (ExMachG Σ Hinv' exm_mem_inG exm_disk_inG)
+                                               }}).
 
   Context (init_absr: Λa.(State) → ExMach.State → Prop).
+  Context (init_wf: ∀ σ1a σ1c, init_absr σ1a σ1c → state_wf σ1c).
 
-  Context (init_inv: ∀ σ1a σ1c ρ, init_absr σ1a σ1c →
+  Context (init_exec_inner: ∀ σ1a σ1c ρ, init_absr σ1a σ1c →
       (∀ `{Hex: exmachG Σ} `{Hcfg: cfgG OpT Λa Σ},
-          (([∗ map] i ↦ v ∈ mem_state σ1c, i m↦ v) -∗
-           ([∗ map] i ↦ v ∈ disk_state σ1c, i d↦ v) -∗
-           source_ctx (ρ, σ1a) ∗ source_state σ1a) ={⊤}=∗ φinv _ _)).
+          (([∗ map] i ↦ v ∈ mem_state σ1c, i m↦ v) ∗
+           ([∗ map] i ↦ v ∈ disk_state σ1c, i d↦ v) ∗
+           source_ctx (ρ, σ1a) ∗ source_state σ1a) ={⊤}=∗ exec_inner _ _)).
 
+  (*
   Context (inv_preserve_crash:
       (∀ `{Hex: exmachG Σ} `{Hcfg: cfgG OpT Λa Σ},
           (∃ Hinv H0', @φinv Hcfg (@ExMachG Σ Hinv H0' (exm_disk_inG))) -∗
           ([∗ map] i ↦ v ∈ init_zero, i m↦ v) ={⊤}=∗ φinv _ _)).
+   *)
 
+  Context (exec_inv_preserve_crash:
+      (∀ `{Hex: exmachG Σ} `{Hcfg: cfgG OpT Λa Σ},
+          exec_inv Hcfg Hex ={⊤, E}=∗ ∀ Hmem',
+          (let Hex := ExMachG Σ (exm_invG) Hmem' (exm_disk_inG) in
+              ([∗ map] i ↦ v ∈ init_zero, i m↦ v) ={E}=∗ crash_inner Hcfg Hex))).
+
+  Context (crash_inv_preserve_crash:
+      (∀ `{Hex: exmachG Σ} `{Hcfg: cfgG OpT Λa Σ},
+          crash_inv Hcfg Hex ={⊤, E}=∗ ∀ Hmem',
+          (let Hex := ExMachG Σ (exm_invG) Hmem' (exm_disk_inG) in
+              ([∗ map] i ↦ v ∈ init_zero, i m↦ v) ={E}=∗ crash_inner Hcfg Hex))).
+
+  (* TODO: Much of this business is just to capture the fact that exec_inner/crash_inner
+     should not really mention invariants, because those old invariants are 'dead' *)
+  Context (crash_inner_inv :
+      (∀ `{Hex: exmachG Σ} `{Hcfg: cfgG OpT Λa Σ},
+          (∃ Hinv, crash_inner Hcfg (ExMachG Σ Hinv (exm_mem_inG) (exm_disk_inG)))
+          ={⊤}=∗ crash_inv Hcfg Hex)).
+
+  Context (exec_inner_inv :
+      (∀ `{Hex: exmachG Σ} `{Hcfg: cfgG OpT Λa Σ} Hinv,
+          exec_inner Hcfg (ExMachG Σ Hinv (exm_mem_inG) (exm_disk_inG))
+          ={⊤}=∗ exec_inv Hcfg Hex)).
+
+  Context (inv_implies_source:
+             ∀ `{Hex: exmachG Σ} `{Hcfg: cfgG OpT Λa Σ},
+             exec_inv Hcfg Hex ={⊤, E}=∗ ∃ σ2a : Λa.(State), source_state σ2a).
+
+  (* TODO: should we model explicit effects of finishing programs? *)
+  Context (exec_inv_preserve_finish:
+      (∀ `{Hex: exmachG Σ} `{Hcfg: cfgG OpT Λa Σ},
+          exec_inv Hcfg Hex ={⊤, E}=∗ ∃ σ2a : Λa.(State), source_state σ2a ∗
+          ∀ `{Hcfg': cfgG OpT Λa Σ} (Hinv': invG Σ) ρ,
+            source_ctx (ρ, σ2a) ∗ source_state σ2a  ={⊤}=∗
+             exec_inner Hcfg' (ExMachG Σ Hinv' exm_mem_inG exm_disk_inG))).
+
+
+  Lemma exmach_crash_refinement_seq {T} σ1c σ1a (es: proc_seq OpT T) :
+    init_absr σ1a σ1c →
+    ¬ proc_exec_seq Λa es (rec_singleton (Ret ())) σ1a Err →
+    ∀ σ2c res, ExMach.l.(proc_exec_seq) (compile_proc_seq es) (rec_singleton recv) σ1c (Val σ2c res) →
+    ∃ σ2a, Λa.(proc_exec_seq) es (rec_singleton (Ret tt)) σ1a (Val σ2a res).
+  Proof.
+    rewrite /compile_proc_seq. intros Hinit Hno_err.
+    unshelve (eapply wp_proc_seq_refinement_adequacy with
+                  (φ := fun _ _ _ => True%I)
+                  (φrec := fun _ _ => True%I)
+                  (E0 := E); eauto).
+    clear Hno_err.
+    iAssert (∀ invG H1 ρ, |={⊤}=>
+         ∃ hM hD
+              (Hmpf_eq : hM.(@gen_heap_inG addr nat Σ nat_eq_dec nat_countable) =
+            H.(@exm_preG_disk Σ).(@gen_heap_preG_inG addr nat Σ nat_eq_dec nat_countable))
+              (Hdpf_eq : hD.(@gen_heap_inG addr nat Σ nat_eq_dec nat_countable) =
+            H.(@exm_preG_disk Σ).(@gen_heap_preG_inG addr nat Σ nat_eq_dec nat_countable)),
+           (@ex_mach_interp _ hM hD σ1c) ∗
+           (source_ctx (ρ, σ1a) -∗ source_state σ1a ={⊤}=∗
+         exec_inner H1 (ExMachG Σ invG hM hD)))%I as "Hpre".
+      {
+        iIntros.
+  iMod (gen_heap_strong_init (mem_state σ1c)) as (hM Hmpf_eq) "(Hmc&Hm)".
+  iMod (gen_heap_strong_init (disk_state σ1c)) as (hD Hdpf_eq) "(Hdc&Hd)".
+  iModIntro. iExists hM, hD, Hmpf_eq, Hdpf_eq. iSplitL "Hmc Hdc".
+  { iExists _, _. iFrame. iPureIntro.
+    edestruct (init_wf) as (Hwf1&Hwf2); eauto.
+    split_and!; eauto; intros i.
+    * destruct (Hwf1 i); intuition.
+    * destruct (Hwf2 i); intuition.
+  }
+  iIntros.
+  iPoseProof (init_exec_inner σ1a σ1c ρ Hinit (ExMachG Σ _ hM hD) _) as "H".
+  iMod ("H" with "[-]") as "$".
+  { iFrame.  iSplitL "Hm"; [| iSplitL "Hd"].
+    { rewrite -Hmpf_eq. iApply mem_init_to_bigOp; auto. }
+    { rewrite -Hdpf_eq. iApply disk_init_to_bigOp; auto. }
+    eauto.
+  }
+  eauto.
+  }
+
+  clear Hinit.
+    iInduction es as [|es] "IH" forall (σ1a σ1c) "Hpre".
+    -
+
+      iSplit; first by eauto.
+  iExists (fun cfgG s => ∃ (_ : exmachG Σ),
+                     state_interp s ∗
+                       (∃ (hM: gen_heapG addr nat Σ)
+                            (Hmpf_eq : hM.(@gen_heap_inG addr nat Σ nat_eq_dec nat_countable) =
+                                       H.(@exm_preG_disk Σ).(@gen_heap_preG_inG addr nat Σ nat_eq_dec nat_countable)) ,
+            gen_heap_ctx init_zero ∗ crash_inner cfgG (ExMachG Σ _ hM (exm_disk_inG))))%I; auto.
+  iIntros (invG0 Hcfg0).
+  iMod ("Hpre" $! invG0 _ _) as (hM hD ??) "(Hstate0&H)".
+  iExists (@ex_mach_interp _ hM hD).
+  iIntros "!> (#Hsrc&Hpt0&Hstate)".
+  iMod ("H" with "Hsrc Hstate") as "Hinv".
+  iMod (exec_inner_inv (ExMachG Σ _ hM hD) _ with "Hinv") as "#Hinv".
+  simpl.
+  iModIntro.
+  iFrame "Hstate0".
+  iSplitL "Hpt0".
+  {  iPoseProof (@wp_mono with "[Hpt0]") as "H"; swap 1 2.
+     { iApply refinement_triples. iFrame. iFrame "Hinv". }
+     { reflexivity. }
+     iApply (wp_wand with "H [Hinv]").
+     iIntros (v) "Hpt0". iFrame.
+     iIntros (σ2c) "Hmach".
+     iMod (inv_implies_source with "Hinv") as (σ2a) "H".
+     iModIntro. iExists _; iFrame; auto.
+  }
+  iSplit.
+  { iIntros (σ2c) "Hmach".
+    iMod (exec_inv_preserve_crash with "Hinv") as "Hinv_post".
+    iMod (gen_heap_strong_init (init_zero)) as (hM' Hmpf_eq') "(Hmc&Hm)".
+    iMod ("Hinv_post" with "[Hm]") as "Hinv'".
+    { rewrite -Hmpf_eq'. iApply @mem_init_to_bigOp; auto. }
+    iIntros. iModIntro.
+    iExists (ExMachG Σ _ hM hD). iFrame "Hmach".
+    iExists hM', Hmpf_eq'. iFrame.
+  }
+  iModIntro. iIntros (invG Hcfg' ?? Hcrash) "Hinv0".
+  iDestruct "Hinv0" as (HexmachG') "(Hinterp&Hinv0)".
+  iDestruct "Hinv0" as (hM' Hmpf_eq') "(Hmc'&Hcrash_inner)".
+  iClear "Hinv".
+  iMod (crash_inner_inv (ExMachG Σ _
+                                 hM' (exm_disk_inG)) Hcfg'
+                         with "[Hcrash_inner]") as "#Hinv".
+  { iIntros. simpl. iExists ( exmachG_irisG.(@iris_invG Op ExMach.State Σ)).
+    iFrame. }
+  iModIntro.
+  iExists (@ex_mach_interp Σ hM' (exm_disk_inG)).
+  iSplitL "Hinterp Hmc'".
+  { (* shows ex_mach_interp is holds after crash for next gen *)
+    rewrite /ex_mach_interp.
+    iDestruct "Hinterp" as (mems disks) "(Hdisks&?&%&Hp)".
+    iDestruct "Hp" as %(Hdisks&Hwf1'&Hwf2').
+    inversion Hcrash; subst.
+    iExists init_zero, _.
+    iFrame.
+    iPureIntro. split_and!.
+    * rewrite /crash_fun//=.
+    * rewrite /crash_fun//=.
+    * rewrite /crash_fun/=. intros i Hsome.
+      apply not_le; intros Hge.
+      rewrite init_zero_lookup_ge_None in Hsome; last by lia.
+      apply is_Some_None in Hsome; auto.
+    * rewrite /crash_fun; auto.
+  }
+  iSplitL "Hinv".
+  {
+    iPoseProof (@wp_mono with "[Hinv]") as "H"; swap 1 2.
+    { iApply recv_triple. iApply "Hinv". }
+    { reflexivity. }
+    iApply (@wp_mono with "H").
+    iIntros (_) "H". iIntros (σ2c) "Hinterp".
+    iMod "H". iModIntro.
+    iDestruct "H" as (σ2a σ2a') "(Hsource&Hinner&Hp)".
+    iExists _, _. iFrame.
+  }
+  {
+    iIntros (σ2c) "Hmach".
+    iMod (crash_inv_preserve_crash with "Hinv") as "Hinv_post".
+    iMod (gen_heap_strong_init (init_zero)) as (hM'' Hmpf_eq'') "(Hmc&Hm)".
+    iMod ("Hinv_post" with "[Hm]") as "Hinv'".
+    { rewrite -Hmpf_eq''. iApply @mem_init_to_bigOp; auto. }
+    iIntros. iModIntro.
+
+    iExists {| exm_invG := invG;
+               exm_mem_inG := hM';
+               exm_disk_inG := HexmachG'.(@exm_disk_inG Σ) |}.
+    iFrame. iExists hM'', Hmpf_eq''. iFrame.
+  }
+  -
+    iSplit; first by eauto.
+  iExists (fun cfgG s => ∃ (Hex : exmachG Σ),
+                     state_interp s ∗
+                       (∃ (hM: gen_heapG addr nat Σ)
+                            (Hmpf_eq : hM.(@gen_heap_inG addr nat Σ nat_eq_dec nat_countable) =
+                                       H.(@exm_preG_disk Σ).(@gen_heap_preG_inG addr nat Σ nat_eq_dec nat_countable))
+
+                            (Hdpf_eq : (@exm_disk_inG Σ Hex).(@gen_heap_inG addr nat Σ nat_eq_dec nat_countable)=
+                                       H.(@exm_preG_disk Σ).(@gen_heap_preG_inG addr nat Σ nat_eq_dec nat_countable)) ,
+            gen_heap_ctx init_zero ∗ crash_inner cfgG (ExMachG Σ _ hM (exm_disk_inG))))%I; auto.
+  iIntros (invG0 Hcfg0).
+  iMod ("Hpre" $! invG0 _ _) as (hM hD ??) "(Hstate0&H)".
+  iExists (@ex_mach_interp _ hM hD).
+  iIntros "!> (#Hsrc&Hpt0&Hstate)".
+  iMod ("H" with "Hsrc Hstate") as "Hinv".
+  iMod (exec_inner_inv (ExMachG Σ _ hM hD) _ with "Hinv") as "#Hinv".
+  simpl.
+  iModIntro.
+  iFrame "Hstate0".
+  iSplitL "Hpt0".
+  {  iPoseProof (@wp_mono with "[Hpt0]") as "H"; swap 1 2.
+     { iApply refinement_triples. iFrame. iFrame "Hinv". }
+     { reflexivity. }
+     iApply (wp_wand with "H [Hinv]").
+     iIntros (v) "Hpt0". iFrame.
+     iIntros (σ2c) "Hmach".
+     iMod (exec_inv_preserve_finish with "Hinv") as (σ2a) "(H&Hfinish)".
+     iModIntro. iExists _; iFrame; auto.
+     simpl.
+     rewrite -/wp_proc_seq_refinement.
+     iApply "IH".
+     { iIntros. iModIntro.
+       iExists hM. iExists hD. unshelve (iExists _, _); try eauto.
+       iFrame. iIntros. iMod ("Hfinish" with "[-]"). iFrame. eauto.
+       iModIntro. eauto.
+     }
+  }
+  iSplit.
+  { iIntros (σ2c) "Hmach".
+    iMod (exec_inv_preserve_crash with "Hinv") as "Hinv_post".
+    iMod (gen_heap_strong_init (init_zero)) as (hM' Hmpf_eq') "(Hmc&Hm)".
+    iMod ("Hinv_post" with "[Hm]") as "Hinv'".
+    { rewrite -Hmpf_eq'. iApply @mem_init_to_bigOp; auto. }
+    iIntros. iModIntro.
+    iExists (ExMachG Σ _ hM hD). iFrame "Hmach".
+    iExists hM', Hmpf_eq', H2. iFrame.
+  }
+  iModIntro. iIntros (invG Hcfg' ?? Hcrash) "Hinv0".
+  iDestruct "Hinv0" as (HexmachG') "(Hinterp&Hinv0)".
+  iDestruct "Hinv0" as (hM' Hmpf_eq' Hmdpf_eq') "(Hmc'&Hcrash_inner)".
+  iClear "Hinv".
+  iMod (crash_inner_inv (ExMachG Σ _
+                                 hM' (exm_disk_inG)) Hcfg'
+                         with "[Hcrash_inner]") as "#Hinv".
+  { iIntros. simpl. iExists ( exmachG_irisG.(@iris_invG Op ExMach.State Σ)).
+    iFrame. }
+  iModIntro.
+  iExists (@ex_mach_interp Σ hM' (exm_disk_inG)).
+  iSplitL "Hinterp Hmc'".
+  { (* shows ex_mach_interp is holds after crash for next gen *)
+    rewrite /ex_mach_interp.
+    iDestruct "Hinterp" as (mems disks) "(Hdisks&?&%&Hp)".
+    iDestruct "Hp" as %(Hdisks&Hwf1&Hwf2).
+    inversion Hcrash; subst.
+    iExists init_zero, _.
+    iFrame.
+    iPureIntro. split_and!.
+    * rewrite /crash_fun//=.
+    * rewrite /crash_fun//=.
+    * rewrite /crash_fun/=. intros i Hsome.
+      apply not_le; intros Hge.
+      rewrite init_zero_lookup_ge_None in Hsome; last by lia.
+      apply is_Some_None in Hsome; auto.
+    * rewrite /crash_fun; auto.
+  }
+  iSplitL "Hinv".
+  {
+    iPoseProof (@wp_mono with "[Hinv IH]") as "H"; swap 1 2.
+    { iApply recv_triple. iApply "Hinv". }
+    { reflexivity. }
+    iApply (@wp_wand with "H [IH]").
+    iIntros (_) "H". iIntros (σ2c) "Hinterp".
+    iMod "H". iModIntro.
+    iDestruct "H" as (σ2a σ2a') "(Hsource&Hinner&Hfinish)".
+    iExists _, _. iFrame.
+     rewrite -/wp_proc_seq_refinement.
+     iApply "IH".
+     { iIntros. iModIntro.
+       iExists hM'. iExists (HexmachG'.(@exm_disk_inG Σ)). unshelve (iExists _; iExists _); eauto.
+       iFrame "Hinterp".
+       iIntros.
+       iMod ("Hfinish" with "[-]"). iFrame. eauto.
+       iModIntro. eauto.
+     }
+  }
+  {
+    iIntros (σ2c) "Hmach".
+    iMod (crash_inv_preserve_crash with "Hinv") as "Hinv_post".
+    iMod (gen_heap_strong_init (init_zero)) as (hM'' Hmpf_eq'') "(Hmc&Hm)".
+    iMod ("Hinv_post" with "[Hm]") as "Hinv'".
+    { rewrite -Hmpf_eq''. iApply @mem_init_to_bigOp; auto. }
+    iIntros. iModIntro.
+
+    iExists {| exm_invG := invG;
+               exm_mem_inG := hM';
+               exm_disk_inG := HexmachG'.(@exm_disk_inG Σ) |}.
+    iFrame. unshelve (iExists hM'', Hmpf_eq'', _); eauto. iFrame.
+  }
+  Qed.
 
 End refinement.
 
